LogRel/PseudoType.v
@@ -1,4 +1,5 @@
 Require Import Stlc.SpecSyntax.
+Require Import Stlc.SpecTyping.
 Require Import UVal.UVal.
 
 Inductive Prec : Set :=
@@ -19,6 +20,16 @@ Inductive PEnv : Set :=
 
 Notation "Γ p▻ T" := (pevar Γ T) (at level 55, left associativity).
 
+Reserved Notation "⟪  i : T p∈ Γ  ⟫"
+  (at level 0, i at level 98, Γ at level 98).
+Inductive GetEvarP : PEnv → Ix → PTy → Prop :=
+  | GetEvarHere {Γ T} :
+      ⟪   O : T p∈ Γ p▻ T  ⟫
+  | GetEvarThere {Γ T T' i} :
+      ⟪   i : T p∈ Γ      ⟫ →
+      ⟪ S i : T p∈ Γ p▻ T' ⟫
+where "⟪  i : T p∈ Γ  ⟫" := (GetEvarP Γ i T).
+
 Fixpoint repEmul (τ : PTy) : Ty :=
   match τ with
     | ptarr τ₁ τ₂ => tarr (repEmul τ₁) (repEmul τ₂)
@@ -34,3 +45,12 @@ Fixpoint repEmulCtx (Γ : PEnv) : Env :=
     | pempty => empty
     | pevar Γ τ => evar (repEmulCtx Γ) (repEmul τ)
   end.
+
+Lemma getevar_repEmulCtx {i τ Γ} :
+  ⟪ i : τ ∈ repEmulCtx Γ ⟫ →
+  exists τ', ⟪ i : τ' p∈ Γ ⟫ ∧ τ = repEmul τ'.
+Proof.
+  revert i. induction Γ as [|Γ IHΓ τ'']; 
+  inversion 1; [idtac| destruct (IHΓ _ H4) as [? [? ?]]];
+  eauto using GetEvarP.
+Qed.
